src/OCL_main.thy
@@ -43,11 +43,6 @@
 theory OCL_main
 imports OCL_lib OCL_state OCL_tools
 begin
- 
-ML{*
-
-
-*}
 
 (* legacy---still better names ?
 lemmas defined_charn = foundation16
